# DZ 10

## 1
a)
$f(x) = \frac{x^2 + 3e^x}{e^{2x}} = \frac{x^2 +3\displaystyle\sum_{k=1}^{n}\frac{x^k}{k!} + o(x^n)}{\displaystyle\sum_{k=1}^{n}\frac{(2x)^k}{k!}+o(x^n)}=\displaystyle\sum^{n}_{k=1}\frac{3}{2^k}+\frac{k!}{(2x)^{k-2}} + o(x^n)$

b)

$f(x) = x\sqrt[3]{4-4x+x^2}=x\sqrt[3]{(x-2)^2}$

$f'(x) = (x-2)^{2/3} + \frac{2x}{3\sqrt[3]{x-2}} = \frac{3(x-2) + 2x}{3\sqrt[3]{x-2}}=\frac{5x-6}{\sqrt[3]{x-2}}$

$(\sqrt[3]{x-2})' = \frac{1}{3\sqrt[3]{(x-2)^2}}$

$(\sqrt[3]{x-2})'' =  \frac{-2}{6\sqrt[3]{(x-2)^4}}$

$(\sqrt[3]{x-2})^{(n)} = \frac{(-1)^{n+1}}{3\sqrt[3]{(x-2)^{2n}}}$

$f'(x) =27\sqrt[3]{4}x+(5x-6) \displaystyle\sum^{n-1}_{k=1}\frac{3(-1)^{k+1}(-2)^{\frac{2k}{3}}}{k!}x + o(x^n)$

$f(x) = 0 + 27\sqrt[3]{4}x + (15x-18)\displaystyle\sum^{n-1}_{k=1}\frac{(-1)^{k+1}(-2)^{\frac{2k}{3}}}{k!}x + o(x^n)$

## 2

$f(x) = sinxcos2x=\frac{1}{2}(sin(-x)+sin3x)$

$\frac{1}{2}\displaystyle\sum^{n-1}_{k=0}\frac{(-1)^kx^{2k+1}}{(2k+1)!}(-x+3x) + o(x^{2n}) = 
\displaystyle\sum^{n-1}_{k=0}\frac{(-1)^kx^{2k+1}}{(2k+1)!}x + o(x^{2k})$

## 3
$t=x+1$

$f(x) = t^2 2^{(t-1)(t+1)}=t^2 2^{t^2-1}=
t^2 e^{(t^2-1)ln2}$

$e^z = \displaystyle\sum^n_{k=0}\frac{z^k}{k!} + o(z^n)$

$t^2 e^{(t^2-1)ln2}=t^2 \displaystyle\sum_{k=0}^{n+1} \frac{(t^2-1)^kln^k2}{k!} + o(t^{2n+2})$ 

$=(x+1)^2\displaystyle\sum^{n+1}_{k=0}\frac{ln^k2}{k!}x^{2k} + o((x+1)^{2n+1})$

## 4

$f(x) = \sqrt{1+2x-x^2} -\sqrt[3]{1-3x+x^2}$

$t=x-1$

$f(t) = \sqrt{-t^2 +2}-\sqrt[3]{t^3+3t^2-2}$,

$f'(t) = \frac{-t}{\sqrt{2-t^2}}-\frac{t^2+2t}{(t^3+3t-2)^{2/3}}$

$f''(x) = \frac{-\sqrt{2-t^2} +\frac{-t}{\sqrt{2-t^2}}t}{2-t^2} - \frac{(2t+2)(t^3+3t^2-2)^{2/3}-\frac{2(t^2+2t)}{\sqrt[3]{t^3+3^2-2}}}{(t^3+3t-2)^{4/3}}$

$=\frac{-2}{(2-t^2)^{3/2}} -\frac{2(x^4+2x^3-4x^2-4x+2)}{(t^3+3t-2)^{5/3}}$

## 5

$sin(arctg(x))$
