<script type="text/javascript"
  src="https://cdnjs.cloudflare.com/ajax/libs/mathjax/2.7.0/MathJax.js?config=TeX-AMS_CHTML">
</script>
<script type="text/x-mathjax-config">
  MathJax.Hub.Config({
    tex2jax: {
      inlineMath: [['$','$'], ['\\(','\\)']],
      processEscapes: true},
      jax: ["input/TeX","input/MathML","input/AsciiMath","output/CommonHTML"],
      extensions: ["tex2jax.js","mml2jax.js","asciimath2jax.js","MathMenu.js","MathZoom.js","AssistiveMML.js", "[Contrib]/a11y/accessibility-menu.js"],
      TeX: {
      extensions: ["AMSmath.js","AMSsymbols.js","noErrors.js","noUndefined.js"],
      equationNumbers: {
      autoNumber: "AMS"
      }
    }
  });
</script>



# DZ 11

## 1

$(A+Bcosx)sinx = Asinx + Bsinxcosx = Asinx+\frac{B}{2} sin2x  =$

$A \displaystyle\sum^{n=1}_{k=0}\frac{(-1)^kx^{2k + 1}}{(2л+1)!}$
  $+ \frac{B}{2} \displaystyle\sum^{n=1}_{k=0}\frac{(-1)^k + (2x)^{2k + 1}}{(2k + 1)!}$
    $+ o(x^4)$

$= Ax - A\frac{x^3}{6} + Bx - B\frac{2x^3}{3}$

$\begin{cases}
\frac{A}{2}+2B=0\\\\
A+B =1
\end{cases}$

$A=\frac{4}{5}$

$B=\frac{1}{5}$

## 2

$x = \frac{2\pi}{5}$

$f(x) = \displaystyle\sum^n_{k=0}\frac{f^{(k)}(0)}{k!}x^k + \frac{f^{n+1}(\epsilon)}{(n+1)!}x^{n+1} , \epsilon \in (0,x)$

$\epsilon:=\frac{\pi}{3}$


$f(x) = \displaystyle\sum^{n}_{k=0}\frac{(-1)^k}{(2k!)}x^{2k} + \frac{cos^{2n+1}(\frac{\pi}{3})}{(2n+1)!}x^{2n+1}$

$n=1, f(x) \approx 1-\frac{1}{2}\frac{4\pi^2}{25} - \frac{\sqrt3}{2*6}(\frac{2\pi}{5})^3 = 1-\frac{2\pi^2}{25} - \frac{2\sqrt3\pi^3}{375} $

$\frac{2\sqrt3\pi^3}{375} \approx 0.28 > 10^{-3}$

$n=2,f(x) \approx 1 -\frac{1}{2}\frac{4\pi^2}{25} +\frac{1}{24}\frac{16\pi^4}{5^4}  -\frac{\sqrt3}{2*120}\frac{32\pi^5}{5^5}$

$\frac{\sqrt3}{2 * 120}\frac{32 \pi^5}{5^5} = \frac{4 \sqrt3 \pi^5}{15 * 5^5}\approx 0.04 > 10^{-3}$

$n=3,f(x) \approx 1 - \frac{1}{2}\frac{4\pi^2}{25} + \frac{1}{24}\frac{16\pi^4}{5^4} - \frac{1}{720}\frac{64\pi^6}{5^6} - \frac{1}{5040}\frac{128\pi^7}{5^7}$

$\frac{1}{5040}\frac{128\pi^7}{5^7}\approx 0.0009<10^{-3}$

$n=3$ подходит, посчитаем :

$f(x) \approx 0.309$

## 3


$\displaystyle\lim_{x\to 0}\frac{ln(e^{2x}+ sinx)-3arcsinx + \frac{5x^2}{2}}{\sqrt[3]{8+x^3}-2} =$

$
\displaystyle\lim_{x\to 0}\frac{ln(1+2x + 2x^2 +\frac{4x^3}{3}+ o(x^3) + x-\frac{x^3}{6}  + o(x^3)) - 3x-\frac{1}{2}\frac{3x^3}{3}+o(x^3) + \frac{5x^2}{2}}{2\sqrt[3]{1+(\frac{x}{2})^3} -2}$

$\displaystyle\lim_{x\to 0} \frac{ln(1+(3x+2x^2+\frac{7x^3}{6}))-3x-\frac{x^3}{2}+\frac{5x^2}{2}}{2+\frac{1}{3*8}x^3 +o(x^3)-2}$


$\displaystyle\lim_{x\to 0}\frac{3x+\frac{7x^3}{3}-3x-\frac{x^3}{2}+o(x^3)}{\frac{x^3}{24}+o(x^3)}$


$\displaystyle\lim_{x\to 0}\frac{\frac{11x^3}{6}+o(x^3)}{\frac{x^3}{24}+o(x^3)}$

$\displaystyle\lim_{x\to 0}\frac{44x^3}{x^3}=44$

## 4

$\displaystyle_{x\to 0}\frac{\sqrt[3]{1+3x+x^2} + sinln(1-x) - e^{-7x^2/6}}{x-arctgx} =$

$\displaystyle\lim_{x\to 0}\frac{1+x-\frac{2x^2}{3} -\frac{2x^3}{3}+ o(x^3) + sin(-x+\frac{x^2}{2}-\frac{x^3}{3}+o(x^3))-1+\frac{7x^2}{6}}{x-x+\frac{x^3}{3}+o(x^3)}$

$\displaystyle\lim_{x\to 0}\frac{x-\frac{x^2}{2}-\frac{2x^3}{3}+o(x^3) - x+\frac{x^2}{2}-\frac{x^3}{3}+o(x^3)}{\frac{x^3}{3}+o(x^3)}$

$\displaystyle\lim_{x\to 0}\frac{-3x^3+o(x^3)}{x^3+o(x^3)}=-3$


## 5


$\displaystyle\lim_{x\to 0}(\frac{2e^{x-x^2}-2}{2x-x^2})^{\frac{sinx}{x^3}}=$

$\displaystyle\lim_{x\to 0}(2\frac{e^{x-x^2}-1}{2x-x^2})^{\frac{1}{x^2}}=$

$\displaystyle\lim_{x\to 0}(2\frac{1+x-x^2+\frac{(x-x^2)^2}{2}+o(x^2) -1}{2x-x^2})^{\frac{1}{x^2}}=$

$\displaystyle\lim_{x\to 0}(2\frac{x-x^2+\frac{x^2}{2}+o(x^2) }{2x-x^2})^{\frac{1}{x^2}}=$

$\displaystyle\lim_{x\to 0}(2\frac{x-\frac{x^2}{2}+o(x^2) }{2x-x^2})^{\frac{1}{x^2}}=$

$\displaystyle\lim_{x\to 0}(\frac{2x-x^2+o(x^2) }{2x-x^2})^{\frac{1}{x^2}}=$

$\displaystyle\lim_{x\to 0}(1)^{\frac{1}{x^2}}=1$



## 6

$\displaystyle\lim_{x\to\infty}(\frac{\sqrt{x^2-x}}{x}  +\frac{1}{4}sin\frac{2}{x})^{x^2+sin3x}=$

$\displaystyle\lim_{x\to\infty}(\sqrt{1-\frac{1}{x}}  +\frac{1}{4}sin\frac{2}{x})^{x^2+sin3x}$

$t=\frac{1}{x}$

$\displaystyle\lim_{t\to 0}(\sqrt{1-t}+\frac{1}{4}sin2t)^{\frac{1}{t^2}+sin\frac{3}{t}}$

$\displaystyle\lim_{t\to 0}(1+\frac{-t}{2}-\frac{t^2}{8}+o(t^2) +\frac{t}{2}+o(t^2))^{\frac{1}{t^2}+\frac{3}{t}+o(t^2)}=$


$\displaystyle\lim_{t\to 0}(1-\frac{t^2}{8})^{\frac{1}{t^2}}(1-\frac{t^2}{8})^{\frac{3}{t}}=$

$e^{-\frac{1}{8}}((1-\frac{t^2}{8})^{\frac{1}{t^2}})^{3t}=e^{-\frac{1}{8}}(e^{-\frac18})^{3t}=e^{-\frac18}$

## 7

$tgx=\frac{sinx}{cosx}=\frac{1-\frac{\pi^2}{8}+\frac{\pi t}{4}+\frac{t^2}{2}}{x}+o(x^2)$

$t=\frac{\pi}{4}-x$

$\displaystyle\lim_{t\to 0}\frac{ln(ctg(\frac{\pi}{4}-t))-2t}{(1-tgx)^2}=$

$\displaystyle\lim_{t\to 0}\frac{ln(\frac{\frac{\pi}{4}-t}{1-\frac{\pi^2}{8}+\frac{\pi t}{4}+\frac{t^2}{2}}+o(t^2))-2t}{(1-\frac{1-\frac{\pi^2}{8}+\frac{\pi t}{4}+\frac{t^2}{2}}{\frac{\pi}{4}-t})^2}=$

$\displaystyle\lim_{t\to 0}\frac{\frac{\frac{\pi}{4}-t}{1-\frac{\pi^2}{8}+\frac{\pi t}{4}+\frac{t^2}{2}}+o(t^2)-2t}{(\frac{\frac{\pi}{4}-t-1+\frac{\pi^2}{8}-\frac{\pi t}{4}-\frac{t^2}{2}}{\frac{\pi}{4}-t})^2}=$

$\displaystyle\lim_{t\to 0}\frac{\frac{\frac{\pi}{4}-t -2t+\frac{\pi^2t}{4}-\frac{\pi t^4}{2}+o(x^2)}{1-\frac{\pi^2}{8}+\frac{\pi t}{4}+\frac{t^2}{2}}}{(\frac{\frac{\pi}{4}-t-1+\frac{\pi^2}{8}-\frac{\pi t}{4}-\frac{t^2}{2}}{\frac{\pi}{4}-t})^2}=$

$\frac{\pi}{4} * \frac{8}{8-\pi^2} * \frac{16}{(\pi-4)^2} * \frac{\pi^2}{16} = \frac{2\pi^3}{(8-\pi^2)(\pi-4)^2}$