<script type="text/javascript"
  src="https://cdnjs.cloudflare.com/ajax/libs/mathjax/2.7.0/MathJax.js?config=TeX-AMS_CHTML">
</script>
<script type="text/x-mathjax-config">
  MathJax.Hub.Config({
    tex2jax: {
      inlineMath: [['$','$'], ['\\(','\\)']],
      processEscapes: true},
      jax: ["input/TeX","input/MathML","input/AsciiMath","output/CommonHTML"],
      extensions: ["tex2jax.js","mml2jax.js","asciimath2jax.js","MathMenu.js","MathZoom.js","AssistiveMML.js", "[Contrib]/a11y/accessibility-menu.js"],
      TeX: {
      extensions: ["AMSmath.js","AMSsymbols.js","noErrors.js","noUndefined.js"],
      equationNumbers: {
      autoNumber: "AMS"
      }
    }
  });
</script>


# дз 3

## 1

a) $\displaystyle\lim_{n\to \infty} \frac{3n^2 +n-1}{-4n^2-n+3} =\displaystyle\lim_{n\to \infty} \frac{3+ \frac{1}{n}- \frac{1}{n^2}}{-4 - \frac{1}{n} + \frac{3}{n^2}}  = -\frac{3}{4}$

b) $\displaystyle\lim_{n\to \infty} n - \frac{3}{\frac{3}{n} - \frac{3}{n^2}+ \frac{1}{n^3}} =\displaystyle\lim_{n\to \infty} n - \frac{3n^3}{3n^2 - 3n + 1} =\displaystyle\lim_{n\to \infty} \frac{-3n^3 +3n^3 -3n^2 +n}{3n^2 - 3n + 1} =\displaystyle\lim_{n\to \infty} \frac{-3 + \frac{1}{n}}{3 - \frac{3}{n} + \frac{1}{n^2}} = -1$

c)$\displaystyle\lim_{n\to \infty} \frac{2n - \sqrt{4n^2 -1}}{\sqrt{n^2 +3} - n}  =  \displaystyle\lim_{n\to \infty} 2\frac{1 - \sqrt{1 - \frac{1}{4n^2}}}{\sqrt{1 + \frac{3}{n^2}} - 1}= 2$

d) $\displaystyle\lim_{n\to \infty} \sqrt[3]{n+1} - \sqrt[3]{n-1}  = \displaystyle\lim_{n\to \infty} \frac{n+1 -n+1}{(\sqrt[3]{n+1})^2 + \sqrt[3]{(n+1)(n-1)} + (\sqrt[3]{n-1})^2} = 0$

e) $\displaystyle\lim_{n\to \infty} \frac{10^n +n!}{2^n+  (n+1)!} = \displaystyle\lim_{n\to \infty} \frac{\frac{10^n}{n!}+ 1}{\frac{2^n}{n!}+ n+1} = \displaystyle\lim_{n\to \infty} \frac{1}{n+1} =0$

f) $\displaystyle\lim_{n\to \infty} \frac{\sqrt[n]{16} -1}{\sqrt[n]{8} -1} = \displaystyle\lim_{n\to \infty} \frac{ 2^{\frac{4}{n}}-1^4}{2^{\frac{3}{n}} - 1^3}= \displaystyle\lim_{n\to \infty} \frac{(2^{\frac{1}{n}}-1)(2^{\frac{1}{n}}+1)(2^{\frac{2}{n}}+1)}{(2^{\frac{1}{n}}-1)(2^{\frac{2}{n}} + 2^{\frac{1}{n}} + 1)}=\displaystyle\lim_{n\to \infty} \frac{(2^{\frac{1}{n}}+1)(2^{\frac{2}{n}}+1)}{(2^{\frac{2}{n}} + 2^{\frac{1}{n}} + 1)}= \displaystyle\lim_{n\to \infty} \frac{2^{\frac{3}{n}} + 2^{\frac{1}{n}}+ 2^{\frac{2}{n}} + 1}{2^{\frac{2}{n}} + 2^{\frac{1}{n}} + 1} = \displaystyle\lim_{n\to \infty} 1 + \frac{2^{\frac{3}{n}}}{2^{\frac{2}{n}} + 2^{\frac{1}{n}} + 1} = $

$1 + \frac{1}{3} = \frac{4}{3}$

простите первую строчку переписал неправильно, ответ $\frac{3}{4}$)))

## 2 

$\displaystyle\lim_{n\to \infty} x_n \to -\infty \Leftrightarrow \forall C', \exists N(C'), \forall n> N(C'), x_n<C'$

$x_n+y_n <C' + C$

$\forall C'+C, \exists N(C'+C), \forall n> N(C'+C), x_n+y_n<C'+C \Leftrightarrow \displaystyle\lim_{n\to \infty} (x_n+y_n) \to -\infty$

## 3 

$\displaystyle\lim_{n\to \infty} x_n \to \pm\infty \Leftrightarrow \forall C', \exists N(C'), \forall n> N(C'), |x_n|>|C'|$

$|x_n|y_n >|C'|  C$

$|x_ny_n|>|C'C|$

$\forall C'C, \exists N(C'C), \forall n> N(C'C), |x_ny_n|>|C'C| \Leftrightarrow \displaystyle\lim_{n\to \infty} (x_ny_n) \to \pm\infty$
