# DZ 16

## 1

рассмотрим последовательность $[a_0,a_1,...]$

тогда $\Delta S a = \Delta[a_1,a_2,...] = [a_2-a_1,a_3-a_2...]$

$S\Delta a = S[a_1-a_0,a_2-a_1,...]=[a_2-a_1,a_3-a_2...]$

$\to S\Delta = \Delta S$

## 2

$\Delta^n$ всегда имеет вид

$\Delta^n a_i = \sum^n_kC^n_ka_{i+k}$

тогда $\Delta^t a_m = C^t_0a_m +C_1^ta_{m+1}+\dots$

однако $\forall k>m:a_k=0$

тогда старший коэффициент равен $\alpha$

2)

$m=0:$

$n,2n,3n,4n,...$

$m=1$

$n,n,n,...$

$m\geq 2$

$0,0,0,...$


## 4

$\Delta \frac{a_n}{b_n} = \frac{a_{n+1}}{b_{n+1}} - \frac{a_n}{b_n} = $

$\frac{a_{n+1}b_n - a_nb_{n+1}}{b_{n+1}b_n} = $

$\frac{a_{n+1}b_n - a_nb_{n+1} + b_{n+1}a_{n+1} - b_{n+1}a_{n+1}}{b_{n+1}b_n} = $

$\frac{b_{n}(a_n - a_{n+1}) - a_n(b_{n}-b_{n+1})}{b_{n+1}b_n} = $

$\frac{b_n\Delta a_n - a_n\Delta a_n}{b_{n+1}b_n}$


## 5

$\Delta \frac{n^2}{(-3)^{n}} = \frac{(n+1)^2}{(-3)^{n+1}} - \frac{n^2}{(-3)^n} = $

$\frac{n^2+2n+1+3n^2}{(-3)^{n+1}}=\frac{4n^2+2n+1}{(-3)^{n+1}}$

## 6

$\Delta cos(\alpha n+\beta) = $

$cos(\alpha n + \alpha+\beta)-\cos(\alpha n +\beta)$

$-2sin(\alpha n +\beta+\frac{\alpha}{2})sin(\frac{\alpha}{2})$

## 7

вначале посчитаем

$x^5 - (x+1)^5 = 5x^4-10x^3+10x^2-5x+1$

сложим такие уравнения $\forall x\in\underline{n}$

$n^5 = 5\sum n^4- 10\sum n^3 + 10\sum n^2 -5\sum n+1$

$\sum n^4 = \frac{n^5+10\sum n^3 - 10\sum n^2 + 5\sum n + 1}{5} = $

$\frac{n^5+5\frac{n^2(n+1)^2}{2} - 5\frac{n(n+1)(2n+1)}{3} + 5\frac{n(n+1)}{2} + 1}{5} = $

$\frac{n(n+1)(2n+1)(3n^2-3n+1)}{30}$

## 8

### a)

$\sum \frac{1}{(n-1)(n-3)}=\sum (\frac{1/2}{n+1}-\frac{1/2}{n+3}) = $

$\frac{1}{2} - \frac{1}{6} +
\frac{1}{4}-\frac{1}{8} +
\frac{1}{6} - \dots
 = \frac{1}{2}+\frac{1}{4}-\frac{1}{2n+2}-\frac{1}{2n+4}$

 $n\to\infty: \sum =\frac{3}{4}$

 ### b)

 $\sum(b_n\Delta c_n) = (b_nc_n - b_0c_0)  - \sum c_{n+1}\Delta b_{n}$

 $b_n = n^2$

 $c_n = (-\frac{1}{3})^n = -\frac{3}{4}\Delta(\frac{1}{3})$ (заметим что)

 $\sum\frac{n^2}{(-3)^n} = -\frac{3}{4}\sum n^2 \frac{1}{(-3)^n} = $

 $= -\frac{3}{4}(\frac{n^2}{(-3)^n}-\sum (-\frac{1}{3}^{n+1}(2n+1))) = ...=$

 $=\frac{21}{32} +\frac{8n^2-4n-5}{32(-3)^{n-1}}$

 при $n\to\infty:\sum\to\frac{21}{32}$

 ### c)

 $b_n = sin(\alpha n +\gamma) $; $\gamma = \beta - \frac{\alpha}{2}$

 $\Delta b_n = 2sin\frac{\alpha}{2}cos(\alpha n +\gamma +\frac{\alpha}{2})$

$\Delta b_n = 2sin\frac{\alpha}{2}cos(\alpha n +\beta)$


$cos(\alpha n + \beta) = \frac{\Delta b_n}{2sin\frac{\alpha}{2}}$
