# DZ 1

## 2

$3\sum n^5 = 4(\sum n)^3 - (\sum n)^2$

$3\sum n^5 = \frac{n^3(n+1)^3}{2} - \frac{n^2(n+1)^2}{4}$

$3\sum n^5 = \frac{n^2(n+1)^2(2n^2+2n-1)}{4}$

$\sum n^5 = \frac{n^2(n+1)^2(2n^2+2n-1)}{12}$

$\Delta\sum n^5 =\Delta \frac{n^2(n+1)^2(2n^2+2n-1)}{12}$

$ (n+1)^5 =\frac{(n+1)^2(n+2)^2(2(n+1)^2+2n+1)}{12} -\frac{n^2(n+1)^2(2n^2+2n-1)}{12}$

$ (n+1)^5 =\frac{(n+1)^2((n+2)^2(2(n+1)^2+2n+1) - n^2(2n^2+2n-1))}{12}$

$ (n+1)^3 =\frac{((n^2+2n+4)(2n^2+6n+3) - n^2(2n^2+2n-1))}{12}$

$ (n+1)^3 =\frac{12(n+1)^3}{12}$

## 3



