<script type="text/javascript"
  src="https://cdnjs.cloudflare.com/ajax/libs/mathjax/2.7.0/MathJax.js?config=TeX-AMS_CHTML">
</script>
<script type="text/x-mathjax-config">
  MathJax.Hub.Config({
    tex2jax: {
      inlineMath: [['$','$'], ['\\(','\\)']],
      processEscapes: true},
      jax: ["input/TeX","input/MathML","input/AsciiMath","output/CommonHTML"],
      extensions: ["tex2jax.js","mml2jax.js","asciimath2jax.js","MathMenu.js","MathZoom.js","AssistiveMML.js", "[Contrib]/a11y/accessibility-menu.js"],
      TeX: {
      extensions: ["AMSmath.js","AMSsymbols.js","noErrors.js","noUndefined.js"],
      equationNumbers: {
      autoNumber: "AMS"
      }
    }
  });
</script>


# DZ 11

## 1

$(\frac{1=i\sqrt3}{2})^n  = (\frac{1}{2}-i\frac{\sqrt3}{2})^n = (cos(-\frac{\pi}{3})+isin(-\frac{\pi}{3}))^n = 
cos(-\frac{n\pi}{3})+isin(-\frac{n\pi}{3})$

## 2

$(cosx+isinx)^5 = cos5x+isin5x$

$(cosx+isinx)^5 = cos^5x +5icos^4xsix+10i^2cos^3xsin^2x+10i^3cos^2xsin^3x + 5i^4cosxsin^4x + i^5sin^5x = $

$
cos^5x +5icos^4xsix-10cos^3xsin^2x-10icos^2xsin^3x + 5cosxsin^4x + isin^5x = $

$
(cos^5x-10cos^3xsin^2x + 5cosxsin^4x)+ i(5cos^4xsins -10cos^2xsin^3x+isin^5x)$

$cos5x +isin5x = (cos^5x-10cos^3xsin^2x + 5cosxsin^4x)+ i(5cos^4xsins -10cos^2xsin^3x+isin^5x)$

$cos5x = cos^5x-10cos^3xsin^2x + 5cosxsin^4x = 
cos^5 - 10cos^3(1-cos^2x)+5cosx(1-cos^2x)^2 = $

$
cos^5x - 10cos^3x + 10cos^5x +5cosx-10cos^3x+5cos^5x = 16cos^5x-20cos^3x+5cosx$

## 3

$\sqrt[4]{-4}=\sqrt[4]4(cos\frac{\pi+2\pi k}{4}+isin\frac{\pi+2\pi k}{4})  = 
\begin{bmatrix}
\sqrt2(cos\frac{\pi}{4}+isin\frac{\pi}{4})\\\\
\sqrt2(cos\frac{3\pi}{4}+isin\frac{3\pi}{4})\\\\
\sqrt2(cos\frac{5\pi}{4}+isin\frac{5\pi}{4})\\\\
\sqrt2(cos\frac{7\pi}{4}+isin\frac{7\pi}{4})\\\\
\end{bmatrix} = 
\begin{bmatrix}
1+i\\\\
1-i\\\\
-1+i\\\\
-1-i\\\\
\end{bmatrix}$

## 4

$\sqrt[6]{64}=\sqrt[6]{64}(cos\frac{2\pi k}{6} + isin\frac{2\pi k}{6}) = 
\begin{bmatrix}
2(1+0i)\\\\
2(\frac{1}{2}+i\frac{\sqrt3}{2})\\\\
2(-\frac{1}{2}+i\frac{\sqrt3}{2}) \\\\
2(-1+i0) \\\\
2(-\frac{1}{2}+-i\frac{\sqrt3}{2}) \\\\
2(\frac{1}{2}-i\frac{\sqrt3}{2})
\end{bmatrix}=
\begin{bmatrix}
2\\\\2+2i\sqrt3 \\\\-2+2i\sqrt3\\\\-2\\\\-2-2i\sqrt3\\\\2-2i\sqrt3
\end{bmatrix}$

## 5

$ \sqrt[3]{2-2i} = (2(\frac{\sqrt2}{2} - i\frac{\sqrt2}{2}))^{\frac{1}{3}} = \sqrt[3]2(cos\frac{-\pi+8\pi k}{4*3}+isin\frac{-\pi +8\pi k }{4*3}) = $

$
\begin{bmatrix}
\sqrt[3]2(cos\frac{-\pi}{12}+isin\frac{-\pi}{12}) \\\\
\sqrt[3]2(cos\frac{7\pi}{12}+isin\frac{7\pi}{12}) \\\\
\sqrt[3]2(-\frac{\sqrt2}{2}+i\frac{\sqrt2}{2}) \\\\
\end{bmatrix}$

## 6

$(z+1)^n -(z-1)^n=0$

Пусть $z=cos2a +isin2a$

Тогда $z+1 = cos2a+isin2a +1=2cos^2a -1 +i2sinacosa+1=2cos^2a+2isinacosa$

a $z-1= cos2a+isin2a +1=1-2sin^2a +i2sinacosa+1=-(2sin^2a-2isinacosa)$

$\frac{z+1}{z-1} = -\frac{2cos^2a+2isinacosa}{2sin^2a-2isinacosa}=-\frac{cosa(cosa-isina)}{-isina(-isina+icosa)} = \frac{cosa}{isina}=-ictga$

$(\frac{z+1}{z-1})^n=1$

$\frac{z+1}{z-1} = \sqrt[n]1=cos\frac{2\pi k}{n}+isin\frac{2\pi k}{n}$

$-ictga =cos\frac{2\pi k}{n}+isin\frac{2\pi k}{n}$

$a=arcctg(-\frac{cos\frac{2\pi k}{n}+isin\frac{2\pi k}{n}}{i})$

$z=cos2a +isin2a$
## 7

$256x^8+1=0$

$x=\sqrt[8]{-\frac{1}{256}}=\sqrt[8]{\frac{1}{256}}(cos\frac{2\pi k}{8}+isin\frac{2\pi k}{8}) = 
\begin{bmatrix}
\frac{1}{2}\\\\
\frac{1}{2}(\frac{\sqrt2}{2}+i\frac{\sqrt2}{2}) \\\\
\frac{1}{2}(0+i) \\\\
\frac{1}{2}(-\frac{\sqrt2}{2}+i\frac{\sqrt2}{2}) \\\\
-\frac{1}{2}\\\\
\vdots
\end{bmatrix}$

$256x^8+1 = (x-\frac{1}{2})(x-i\frac{1}{2})(x-\frac{\sqrt2 +i\sqrt2}{4})(x-\frac{-\sqrt2 +i\sqrt2}{4})(x+\frac{1}{2})(x+i\frac{1}{2})(x+\frac{\sqrt2 +i\sqrt2}{4})(x+\frac{-\sqrt2 +i\sqrt2}{4})$

$=(x-\frac{1}{2})(x+\frac{1}{2})(x^2+\frac{1}{4})\frac{4x^2+2\sqrt2x+1}{4}\frac{4x^2 -2\sqrt2x+1}{4}$